Sodium/Lean/Syntax.lean
@@ -1,0 +1,172 @@
+import Sodium.Data.Encodable.WType
+
+namespace Lean
+
+namespace Name
+
+private def Shape := Unit ⊕ String ⊕ Nat
+
+local notation "anonymous%" => Sum.inl ()
+local notation "str% " s => Sum.inr (Sum.inl s)
+local notation "num% " n => Sum.inr (Sum.inr n)
+
+private def Shape.arity : Shape → Nat
+  | anonymous% => 0
+  | str% _ => 1
+  | num% _ => 1
+
+local instance : ∀ s, NeZero (Shape.arity (str% s)) := fun _ => ⟨Nat.one_ne_zero⟩
+local instance : ∀ n, NeZero (Shape.arity (num% n)) := fun _ => ⟨Nat.one_ne_zero⟩
+
+private def f : Name → WType fun i : Shape => Fin i.arity
+  | .anonymous => ⟨anonymous%, Fin.elim0⟩
+  | .str k s => ⟨str% s, fun _ => f k⟩
+  | .num k n => ⟨num% n, fun _ => f k⟩
+
+private def finv : WType (fun i : Shape => Fin i.arity) → Name
+  | ⟨anonymous%, _⟩ => .anonymous
+  | ⟨str% s, fn⟩ => .str (finv (fn 0)) s
+  | ⟨num% n, fn⟩ => .num (finv (fn 0)) n
+
+instance instEncodable : Encodable Name :=
+  haveI : Encodable Shape := by unfold Shape; infer_instance
+  Encodable.ofEquiv f finv (by
+    intro n
+    induction n with
+    | anonymous => simp only [f, finv]
+    | str k s ih => simp only [f, finv, ih]
+    | num k n ih => simp only [f, finv, ih])
+
+end Name
+
+instance SyntaxNodeKind.instEncodable : Encodable SyntaxNodeKind :=
+  inferInstanceAs (Encodable Name)
+
+namespace SourceInfo
+
+private def Shape :=
+  Unit
+  ⊕ Substring × String.Pos × Substring × String.Pos
+  ⊕ String.Pos × String.Pos × Bool
+
+instance instEncodable : Encodable SourceInfo :=
+  haveI : Encodable Shape := by unfold Shape; infer_instance
+  let f : SourceInfo → Shape
+    | .none => .inl ()
+    | .original leading pos trailing endPos => .inr (.inl (leading, pos, trailing, endPos))
+    | .synthetic pos endPos canonical => .inr (.inr (pos, endPos, canonical))
+  let finv : Shape → SourceInfo
+    | .inl _ => .none
+    | .inr (.inl (leading, pos, trailing, endPos)) => .original leading pos trailing endPos
+    | .inr (.inr (pos, endPos, canonical)) => .synthetic pos endPos canonical
+  Encodable.ofEquiv f finv fun n => by induction n <;> rfl
+
+end SourceInfo
+
+namespace Syntax.Preresolved
+
+private def Shape := Name ⊕ Name × List String
+
+instance instEncodable : Encodable Syntax.Preresolved :=
+  haveI : Encodable Shape := by unfold Shape; infer_instance
+  let f : Syntax.Preresolved → Shape
+    | .namespace n => .inl n
+    | .decl n fs => .inr (n, fs)
+  let finv : Shape → Syntax.Preresolved
+    | .inl n => .namespace n
+    | .inr (n, fs) => .decl n fs
+  Encodable.ofEquiv f finv fun n => by induction n <;> rfl
+
+end Syntax.Preresolved
+
+namespace Syntax
+
+private def Shape :=
+  Unit
+  ⊕ SourceInfo × String
+  ⊕ SourceInfo × Substring × Name × List Syntax.Preresolved
+  ⊕ SourceInfo × SyntaxNodeKind × Nat
+
+local notation "missing%" => Sum.inl ()
+local notation "atom% " info ", " s => Sum.inr (Sum.inl ⟨info, s⟩)
+local notation "ident% " info ", " s ", " n ", " pre => Sum.inr (Sum.inr (Sum.inl (info, s, n, pre)))
+local notation "node% " info ", " kind ", " k => Sum.inr (Sum.inr (Sum.inr (info, kind, k)))
+
+private def Shape.arity : Shape → Nat
+  | missing% | atom% _, _ | ident% _, _, _, _ => 0
+  | node% _, _, k => k
+
+private def f : Syntax → WType fun i : Shape => Fin i.arity
+  | .missing => ⟨missing%, Fin.elim0⟩
+  | .atom info s => ⟨atom% info, s, Fin.elim0⟩
+  | .ident info s n pre => ⟨ident% info, s, n, pre, Fin.elim0⟩
+  | .node info kind stx =>
+    if _ : stx.size = 0 then ⟨node% info, kind, 0, Fin.elim0⟩
+    else ⟨node% info, kind, stx.size, fun i => f (stx[i]'i.isLt)⟩
+decreasing_by
+  simp_all only [Syntax.node.sizeOf_spec, gt_iff_lt]
+  have h₁ : sizeOf stx < 1 + sizeOf info + sizeOf stx := by omega
+  have h₂ : sizeOf (stx[i]'i.isLt) < sizeOf stx := by
+    simp_all only [Nat.lt_add_left_iff_pos, Fin.getElem_fin, Array.sizeOf_getElem]
+  omega
+
+private def finv : WType (fun i : Shape => Fin i.arity) → Syntax
+  | ⟨missing%, _⟩ => .missing
+  | ⟨atom% info, s, _⟩ => .atom info s
+  | ⟨ident% info, s, n, pre, _⟩ => .ident info s n pre
+  | ⟨node% info, kind, k, fn⟩ => .node info kind <| (Array.ofFn (n := k) id).map fun i => finv (fn i)
+
+private theorem finv_f_eq : ∀ stx, finv (f stx) = stx := by
+  intro stx
+  have : ∀ n (s : Syntax), sizeOf s < n → finv (f s) = s := by
+    intro n
+    induction n with
+    | zero => intros; omega
+    | succ n ih =>
+      intro s hs
+      cases s <;> try simp only [f, finv]
+      rename_i args
+      if h : args.size = 0 then
+        simp only [h, Array.eq_empty_of_size_eq_zero, List.size_toArray, List.length_nil, f,
+          ↓reduceDIte, finv, Array.ofFn_zero, List.map_toArray, List.map_nil]
+      else
+        rw [dif_neg h, finv]
+        congr
+        ext i
+        . simp only [Array.size_map, Array.size_ofFn]
+        . rename_i h₁ h₂
+          simp only [Array.getElem_map, Array.getElem_ofFn, id_eq]
+          have h_lt : sizeOf args[i] < n := by
+            simp only [Syntax.node.sizeOf_spec] at hs
+            have : sizeOf args[i] < sizeOf args := Array.sizeOf_getElem _ i h₂
+            omega
+          exact ih args[i] h_lt
+  exact this (sizeOf stx + 1) stx (Nat.lt_succ_self _)
+
+instance instEncodable : Encodable Syntax :=
+  haveI : Encodable Shape := by unfold Shape; infer_instance
+  Encodable.ofEquiv f finv finv_f_eq
+
+end Syntax
+
+namespace TSyntax
+
+instance instEncodable {kind : SyntaxNodeKind} : Encodable (TSyntax kind) :=
+  let f (stx : TSyntax kind) : Json := Json.mkObj [(kind.toString, encode stx.raw)]
+  let finv (json : Json) : Option (TSyntax kind) :=
+    match json.getObjVal? kind.toString with
+    | .error _ => none
+    | .ok json =>
+      match decode? (α := Syntax) json with
+      | none => none
+      | some a => some ⟨a⟩
+  Encodable.ofLeftInj f finv (fun x => by cases x; simp only [Json.mkObj_getObjVal?_eq_ok, Encodable.encodek, f, finv])
+
+end TSyntax
+
+#eval show MetaM Unit from do
+  let x ← `(tactic| exact?)
+  println! encode x
+  println! decode? (α := TSyntax `tactic) (encode x)
+
+end Lean
