Sodium/Meta/Syntax.lean
@@ -1,7 +1,0 @@
-import Sodium.Data.Digest
-
-open Lean Meta Elab
-
-namespace Lean.Syntax
-
-end Lean.Syntax
